\documentclass[11pt,fleqn]{article} 
\usepackage[margin=0.8in, head=0.8in]{geometry} 
\usepackage{amsmath, amssymb, amsthm}
\usepackage{fancyhdr} 
\usepackage{palatino, url, multicol}
\usepackage{graphicx} 
\usepackage[all]{xy}
\usepackage{polynom} 
\usepackage{pdfsync}
\usepackage{enumerate}
\usepackage{framed}
\usepackage{setspace, adjustbox}
\usepackage{array%,tikz, pgfplots
}

\usepackage{tikz, pgfplots}
\usetikzlibrary{calc}
%\pgfplotsset{my style/.append style={axis x line=middle, axis y line=
%middle, xlabel={$x$}, ylabel={$y$}, axis equal }}
%
\pagestyle{fancy} 
\lfoot{UAF Calculus I}
\rfoot{3-4 The Chain Rule}


\newcommand{\be}{\begin{enumerate}}
\newcommand{\ee}{\end{enumerate}}

\newcommand{\bi}{\begin{itemize}}
\newcommand{\ei}{\end{itemize}}

\begin{document}
\setlength{\parindent}{0cm}
\renewcommand{\headrulewidth}{0pt}
\newcommand{\blank}[1]{\rule{#1}{0.75pt}}
\renewcommand{\d}{\displaystyle}
\vspace*{-0.7in}
\begin{center}
 {\large{ \sc{Section 3.4 The Chain Rule}}}
\end{center}
\begin{enumerate}
\item For each function $H(x)$ below, write it as a (nontrivial) composition of functions in the form $f(g(x)).$
	\begin{multicols}{2}
	\begin{enumerate}
	\item $H(x)=\tan ( 2-x^4)$
	\item $H(x)=e^{2-2x}$
	\end{enumerate}
	\end{multicols}
\vspace{1in}
\item Complete the Chain Rule (using both types of notation)
	\begin{multicols}{2}
	\begin{itemize}
	\item If $F(x)=f(g(x)),$\\ 
	
	then $F'(x)=$\\
	
	\item If $y=f(u)$ and $u=g(x),$\\ 
	
	then $\frac{dy}{dx}=$\\
	\end{itemize}
	\end{multicols}
\item Find the derivative of the function. You do not need to simplify your answer.
	\begin{enumerate}
	\item $\d{y=\sqrt[3]{4-2x}}$
	\vfill
	\item $\d{f(x)=0.04 \sin(3x+e^x)}$
	\vfill
	\newpage
	\item $\d{x(t)=\frac{e^{-\pi t^2/10}}{100}}$  (\textbf{Don't} use the quotient rule here!)
\vfill
	
	\item $\d{g(x)=\frac{50\sqrt{2}}{x+\tan x}}$ (\textbf{Don't} use the quotient rule here!)
	\vfill
	\end{enumerate}
\item Suppose that $f(x)=x^3,\: g(x)=\cos(x)$ and $h(x)=7+e^x.$
	\begin{enumerate}
	\item Find $\d{F(x)=f(x) \left( g(h(x)) \right),}$ then find its derivative.	
	\vfill
	\item Find $\d{G(x)=f(\:g(x) h(x)\:),}$ then find its derivative.
	\vfill
	\newpage
	\item Find $\d{K(x)=\frac{g(x)}{h(f(x))},}$ then find its derivative.
	\vfill
	\item Find $\d{G(x)=f(g( h(x))),}$ then find its derivative.
	\vfill
	\end{enumerate}
\end{enumerate}
\end{document}